Started 1c)

proj1/proj1.dfy
@@ -1,11 +1,9 @@
-
-
 function sum (a:array<int>, i:int, j:int) :int
 decreases j
 reads a
 requires 0 <= i <= j <= a.Length
-{  
-    if i == j then 
+{
+    if i == j then
         0
     else
         a[j-1] + sum(a, i, j-1)
@@ -20,7 +18,7 @@ ensures s == sum(a, i, j)
 
     while (aux < j)
     invariant i <= aux <= j
-    invariant s == sum(a, i, aux) 
+    invariant s == sum(a, i, aux)
     decreases  j - aux
     {
         s := s + a[aux];
@@ -29,15 +27,34 @@ ensures s == sum(a, i, j)
     return s;
 }
 
-method queryFast (a:array<int>, c:array<int>, i:int, j:int) returns (r:int) 
-requires is_prefix_sum_for(a,c) ∧ // TODO
-ensures // TODO
+
+
+
+
+method queryFast (a:array<int>, c:array<int>, i:int, j:int) returns (r:int)
+requires is_prefix_sum_for(a,c) ∧ 0 <= i <= j <= a.Length ∧ a.Length < c.Length
 {
-    //TODO
+    r:= 0;
+
+    if i == 0{
+        r := c[j - 1];
+    }
+    else {
+        r := c[j-1] - c[i-1];
+    }
+    return r;
 }
 
 predicate is_prefix_sum_for (a:array<int>, c:array<int>)
 reads c, a
 {
-    //TODO
+    var i := c.Length;
+
+    while (i >= 1)
+    invariant 1 <= i <= c.Length
+    decreases i
+    {
+        c[i] == sum(a,0,i-1);
+        i := i - 1;
+    }
 }
